wip/MoreUtils.thy
@@ -1,0 +1,89 @@
+theory MoreUtils
+  imports Main
+begin
+
+unbundle lattice_syntax
+
+
+context boolean_algebra
+begin
+
+definition impl :: "'a \<Rightarrow> 'a \<Rightarrow> 'a" (infixr "\<leadsto>" 60) where
+  "a \<leadsto> b \<equiv> -a \<squnion> b"
+
+lemma impl_shunt:
+  \<open>c \<sqinter> a \<le> b \<longleftrightarrow> c \<le> a \<leadsto> b\<close>
+  by (simp add: impl_def shunt1)
+
+lemma impl_shunt2:
+  \<open>-(a \<leadsto> b) \<le> c \<longleftrightarrow> a \<le> b \<squnion> c\<close>
+  by (simp add: impl_def shunt2)
+
+lemma impl_simps[simp]:
+  \<open>\<top> \<leadsto> b = b\<close>
+  \<open>\<bottom> \<leadsto> b = \<top>\<close>
+  \<open>a \<leadsto> \<bottom> = - a\<close>
+  \<open>a \<leadsto> \<top> = \<top>\<close>
+  \<open>a \<leadsto> a = \<top>\<close>
+  by (force simp add: impl_def)+
+
+definition bequiv :: "'a \<Rightarrow> 'a \<Rightarrow> 'a" (infixr "\<sim>" 60) where
+  "a \<sim> b \<equiv> (a \<leadsto> b) \<sqinter> (b \<leadsto> a)"
+
+lemma bequiv_simps[simp]:
+  \<open>a \<sim> a = \<top>\<close>
+  \<open>a \<sim> -a = \<bottom>\<close>
+  \<open>-a \<sim> a = \<bottom>\<close>
+  \<open>a \<sim> \<top> = a\<close>
+  \<open>\<top> \<sim> a = a\<close>
+  \<open>a \<sim> \<bottom> = -a\<close>
+  \<open>\<bottom> \<sim> a = -a\<close>
+  by (clarsimp simp add: bequiv_def impl_def)+
+
+lemma bequiv_iff: \<open>a \<sim> b = (-a \<squnion> b) \<sqinter> (-b \<squnion> a)\<close>
+  by (simp add: bequiv_def impl_def)
+
+lemma bequiv_iff2: \<open>a \<sim> b = (a \<sqinter> b) \<squnion> (-a \<sqinter> -b)\<close>
+  using bequiv_iff sup.commute sup_inf_distrib2 by force
+
+definition bxor :: "'a \<Rightarrow> 'a \<Rightarrow> 'a" (infixr "\<oplus>" 60) where
+  "a \<oplus> b \<equiv> a \<sqinter> -b \<squnion> -a \<sqinter> b"
+
+lemma bxor_simps[simp]:
+  \<open>a \<oplus> a = \<bottom>\<close>
+  \<open>a \<oplus> -a = \<top>\<close>
+  \<open>-a \<oplus> a = \<top>\<close>
+  \<open>a \<oplus> \<bottom> = a\<close>
+  \<open>\<bottom> \<oplus> a = a\<close>
+  \<open>a \<oplus> \<top> = -a\<close>
+  \<open>\<top> \<oplus> a = -a\<close>
+  by (clarsimp simp add: bxor_def impl_def)+
+
+end
+
+lemma mem_impl_iff[simp]:
+  \<open>x \<in> A \<leadsto> B \<longleftrightarrow> (x \<in> A \<longrightarrow> x \<in> B)\<close>
+  by (simp add: impl_def)
+
+lemma pred_impl_apply[simp]:
+  \<open>(a \<leadsto> b) x = (a x \<longrightarrow> b x)\<close>
+  by (simp add: impl_def)
+
+lemma rel_impl_apply[simp]:
+  \<open>(a \<leadsto> b) x y = (a x y \<longrightarrow> b x y)\<close>
+  by (simp add: impl_def)
+
+lemma mem_bequiv_iff[simp]:
+  \<open>x \<in> A \<sim> B \<longleftrightarrow> (x \<in> A \<longleftrightarrow> x \<in> B)\<close>
+  by (force simp add: bequiv_def)
+
+lemma pred_bequiv_apply[simp]:
+  \<open>(a \<sim> b) x \<longleftrightarrow> (a x = b x)\<close>
+  by (force simp add: bequiv_def)
+
+lemma rel_bequiv_apply[simp]:
+  \<open>(a \<sim> b) x y = (a x y = b x y)\<close>
+  by (force simp add: bequiv_def)
+
+
+end
